src/Ex/MsiSvTopo.v
@@ -1,0 +1,75 @@
+Require Import Bool Vector List String Peano_dec.
+Require Import Common FMap HVector ListSupport Syntax Semantics.
+Require Import Topology RqRsTopo.
+
+Require Import Spec SpecSv Msi MsiSv.
+
+Lemma msiSv_topo_wf: WfDTree topo.
+Proof.
+  split.
+  - compute; repeat constructor; firstorder.
+  - compute; repeat constructor; firstorder.
+Qed.
+
+Lemma msiSv_impl_RqRsChnsOnDTree: RqRsChnsOnDTree topo impl.
+Proof.
+  (** TODO: extensionality for [DTree] w.r.t. [oidx] *)
+Admitted.
+
+Lemma msiSv_impl_RqRsDTree: RqRsDTree topo impl.
+Proof.
+  split.
+  - auto using msiSv_topo_wf.
+  - auto using msiSv_impl_RqRsChnsOnDTree.
+Qed.
+
+Lemma msiSv_impl_GoodRqRsSys: GoodRqRsSys topo impl.
+Proof.
+  repeat
+    match goal with
+    | [ |- GoodRqRsSys _ _] => red
+    | [ |- Forall _ _] => constructor; simpl
+    | [ |- GoodRqRsObj _ _ _] => red
+    end.
+
+  - left.
+    repeat
+      (match goal with
+       | [H: (_ /\oprec _) _ _ _ |- _] => destruct H
+       | [H: rule_precond _ _ _ _ |- _] => simpl in H
+       | [H: rule_trs _ _ _ _ = _ |- _] => simpl in H
+       | [H: (_, _) = (_, _) |- _] => inv H
+
+       | [ |- RulePrecSat _ _] => red
+       | [ |- RulePostSat _ _] => red; intros
+       | [ |- RsReleasing _] => red
+       | [ |- FootprintSilent _] => red
+       | [ |- ImmDownRule _ _ _] => red
+       | [ |- ImmDownOk _ _ _ _ _ _ _ _] => red
+
+       | [ |- _ /\ _] => split
+       | [ |- _ ->oprec _] => red; intros
+       | [ |- Forall _ _] => constructor
+       end; try assumption; try reflexivity).
+
+    red in H.
+    destruct rins as [|[midx msg] [|]]; try discriminate.
+    inv H.
+    
+    exists ext1Idx; do 4 eexists; repeat ssplit; try reflexivity.
+  - 
+    
+Admitted.
+
+Lemma msiSv_impl_RqUpRsUpOkSys: RqUpRsUpOkSys topo impl.
+Proof.
+Admitted.
+
+Theorem msiSv_impl_RqRsSys: RqRsSys topo impl.
+Proof.
+  red; repeat ssplit.
+  - auto using msiSv_impl_RqRsDTree.
+  - auto using msiSv_impl_GoodRqRsSys.
+  - auto using msiSv_impl_RqUpRsUpOkSys.
+Qed.
+
